@prefix : <http://www.owl-ontologies.com/bimxel#> .
@prefix owl: <http://www.w3.org/2002/07/owl#> .
@prefix rdf: <http://www.w3.org/1999/02/22-rdf-syntax-ns#> .
@prefix xml: <http://www.w3.org/XML/1998/namespace> .
@prefix xsd: <http://www.w3.org/2001/XMLSchema#> .
@prefix rdfs: <http://www.w3.org/2000/01/rdf-schema#> .
@base <http://www.owl-ontologies.com/bimxel#> .

<http://www.owl-ontologies.com/bimxel#> rdf:type owl:Ontology ;
                                         owl:imports <https://qudt.org/3.1.5/vocab/quantitykind> ,
                                                     <https://standards.buildingsmart.org/IFC/DEV/IFC4_1/OWL> ;
                                         owl:versionInfo "0.0.1" ;
                                         <https://w3id.org/mod#createdWith> <https://chowlk.linkeddata.es/> .

#################################################################
#    Annotation properties
#################################################################

###  http://www.w3.org/2000/01/rdf-schema#comment
rdfs:comment rdf:type owl:AnnotationProperty ;
             rdfs:label "comment" .


###  http://www.w3.org/2000/01/rdf-schema#label
rdfs:label rdf:type owl:AnnotationProperty ;
           rdfs:label "label" .


###  http://www.w3.org/2002/07/owl#versionInfo
owl:versionInfo rdf:type owl:AnnotationProperty .


###  https://w3id.org/mod#createdWith
<https://w3id.org/mod#createdWith> rdf:type owl:AnnotationProperty .


#################################################################
#    Object Properties
#################################################################

###  http://qudt.org/schema/qudt/hasQuantityKind
<http://qudt.org/schema/qudt/hasQuantityKind> rdf:type owl:ObjectProperty ;
                                              rdfs:label "has quantity kind" .


###  http://www.owl-ontologies.com/bimxel#HasProject
:HasProject rdf:type owl:ObjectProperty ;
            rdfs:domain :BIMxel ;
            rdfs:range :BIMxelProject ;
            rdfs:label "has project" .


###  http://www.owl-ontologies.com/bimxel#IsContainedIn
:IsContainedIn rdf:type owl:ObjectProperty ;
               rdfs:domain :BIMxel ;
               rdfs:comment "Is Contained In."@en ;
               rdfs:label "is contained in" .


###  http://www.w3.org/2004/02/skos/core#broader
<http://www.w3.org/2004/02/skos/core#broader> rdf:type owl:ObjectProperty ;
                                              rdfs:label "broader" .


#################################################################
#    Data properties
#################################################################

###  http://qudt.org/vocab/quantitykind/Power
<http://qudt.org/vocab/quantitykind/Power> rdf:type owl:DatatypeProperty ;
                                           rdfs:domain <http://www.owl-ontologies.com/sosa#Observation> ,
                                                       <http://www.owl-ontologies.com/time#Interval> ;
                                           rdfs:label "power" .


###  http://www.owl-ontologies.com/bot#Element
<http://www.owl-ontologies.com/bot#Element> rdf:type owl:DatatypeProperty ;
                                            rdfs:domain <http://www.owl-ontologies.com/sosa#Observation> ,
                                                        <http://www.owl-ontologies.com/time#Interval> .


###  http://www.owl-ontologies.com/bot#Space
<http://www.owl-ontologies.com/bot#Space> rdf:type owl:DatatypeProperty ;
                                          rdfs:domain <http://www.owl-ontologies.com/sosa#Observation> .


###  http://www.owl-ontologies.com/bot#Zone
<http://www.owl-ontologies.com/bot#Zone> rdf:type owl:DatatypeProperty ;
                                         rdfs:domain <http://www.owl-ontologies.com/bot#Element> .


###  http://www.owl-ontologies.com/sosa#Observation
<http://www.owl-ontologies.com/sosa#Observation> rdf:type owl:DatatypeProperty ;
                                                 rdfs:domain <http://www.owl-ontologies.com/bot#Element> ,
                                                             <http://www.owl-ontologies.com/bot#Space> ,
                                                             <http://www.owl-ontologies.com/bot#Zone> ,
                                                             <http://www.owl-ontologies.com/time#Instant> ,
                                                             <http://www.owl-ontologies.com/time#Interval> .


###  http://www.owl-ontologies.com/time#Instant
<http://www.owl-ontologies.com/time#Instant> rdf:type owl:DatatypeProperty ;
                                             rdfs:domain <http://www.owl-ontologies.com/bot#Element> ,
                                                         <http://www.owl-ontologies.com/sosa#Observation> .


###  http://www.owl-ontologies.com/time#Interval
<http://www.owl-ontologies.com/time#Interval> rdf:type owl:DatatypeProperty ;
                                              rdfs:domain <http://www.owl-ontologies.com/bot#Space> ,
                                                          <http://www.owl-ontologies.com/bot#Zone> ,
                                                          <http://www.owl-ontologies.com/sosa#Observation> .


#################################################################
#    Classes
#################################################################

###  http://qudt.org/vocab/quantitykind/AmountOfSubstanceConcentration
<http://qudt.org/vocab/quantitykind/AmountOfSubstanceConcentration> rdf:type owl:Class ;
                                                                    rdfs:label "Amount Of Substance Concentration" .


###  http://qudt.org/vocab/quantitykind/Energy
<http://qudt.org/vocab/quantitykind/Energy> rdf:type owl:Class ;
                                            rdfs:label "Energy" .


###  http://qudt.org/vocab/quantitykind/MoistureContent
<http://qudt.org/vocab/quantitykind/MoistureContent> rdf:type owl:Class ;
                                                     rdfs:label "Moisture Content" .


###  http://qudt.org/vocab/quantitykind/PersonCount
<http://qudt.org/vocab/quantitykind/PersonCount> rdf:type owl:Class ;
                                                 rdfs:label "Person Count" .


###  http://qudt.org/vocab/quantitykind/RelativeHumidity
<http://qudt.org/vocab/quantitykind/RelativeHumidity> rdf:type owl:Class ;
                                                      rdfs:label "Relative Humidity" .


###  http://qudt.org/vocab/quantitykind/Temperature
<http://qudt.org/vocab/quantitykind/Temperature> rdf:type owl:Class ;
                                                 rdfs:label "Temperature" .


###  http://qudt.org/vocab/quantitykind/Volume
<http://qudt.org/vocab/quantitykind/Volume> rdf:type owl:Class ;
                                            rdfs:label "Volume" .


###  http://qudt.org/vocab/quantitykind/VolumetricFlowRate
<http://qudt.org/vocab/quantitykind/VolumetricFlowRate> rdf:type owl:Class ;
                                                        rdfs:label "Volumetric Flow Rate" .


###  http://standards.buildingsmart.org/IFC/DEV/IFC4_1/OWL#IfcBuilding
<http://standards.buildingsmart.org/IFC/DEV/IFC4_1/OWL#IfcBuilding> rdf:type owl:Class ;
                                                                    owl:equivalentClass :BIMxelBuilding ;
                                                                    rdfs:label "Ifc Building" .


###  http://standards.buildingsmart.org/IFC/DEV/IFC4_1/OWL#IfcBuildingStorey
<http://standards.buildingsmart.org/IFC/DEV/IFC4_1/OWL#IfcBuildingStorey> rdf:type owl:Class ;
                                                                          owl:equivalentClass :BIMxelLevel ;
                                                                          rdfs:label "Ifc Building Storey" .


###  http://standards.buildingsmart.org/IFC/DEV/IFC4_1/OWL#IfcElement
<http://standards.buildingsmart.org/IFC/DEV/IFC4_1/OWL#IfcElement> rdf:type owl:Class ;
                                                                   owl:equivalentClass :BIMxelElement ;
                                                                   rdfs:label "Ifc Element" .


###  http://standards.buildingsmart.org/IFC/DEV/IFC4_1/OWL#IfcProject
<http://standards.buildingsmart.org/IFC/DEV/IFC4_1/OWL#IfcProject> rdf:type owl:Class ;
                                                                   owl:equivalentClass :BIMxelProject ;
                                                                   rdfs:label "Ifc Project" .


###  http://standards.buildingsmart.org/IFC/DEV/IFC4_1/OWL#IfcSite
<http://standards.buildingsmart.org/IFC/DEV/IFC4_1/OWL#IfcSite> rdf:type owl:Class ;
                                                                owl:equivalentClass :BIMxelSite ;
                                                                rdfs:label "Ifc Site" .


###  http://standards.buildingsmart.org/IFC/DEV/IFC4_1/OWL#IfcSpace
<http://standards.buildingsmart.org/IFC/DEV/IFC4_1/OWL#IfcSpace> rdf:type owl:Class ;
                                                                 owl:equivalentClass :BIMxelSpace ;
                                                                 rdfs:label "Ifc Space" .


###  http://www.owl-ontologies.com/bimxel#BIMxel
:BIMxel rdf:type owl:Class ;
        rdfs:label "B I Mxel" .


###  http://www.owl-ontologies.com/bimxel#BIMxelBuilding
:BIMxelBuilding rdf:type owl:Class ;
                rdfs:label "B I Mxel Building" .


###  http://www.owl-ontologies.com/bimxel#BIMxelElement
:BIMxelElement rdf:type owl:Class ;
               rdfs:label "B I Mxel Element" .


###  http://www.owl-ontologies.com/bimxel#BIMxelLevel
:BIMxelLevel rdf:type owl:Class ;
             rdfs:label "B I Mxel Level" .


###  http://www.owl-ontologies.com/bimxel#BIMxelProject
:BIMxelProject rdf:type owl:Class ;
               rdfs:label "B I Mxel Project" .


###  http://www.owl-ontologies.com/bimxel#BIMxelSite
:BIMxelSite rdf:type owl:Class ;
            rdfs:label "B I Mxel Site" .


###  http://www.owl-ontologies.com/bimxel#BIMxelSpace
:BIMxelSpace rdf:type owl:Class ;
             rdfs:label "B I Mxel Space" .


###  http://www.owl-ontologies.com/bot#Element
<http://www.owl-ontologies.com/bot#Element> rdf:type owl:Class .


###  http://www.owl-ontologies.com/bot#Space
<http://www.owl-ontologies.com/bot#Space> rdf:type owl:Class .


###  http://www.owl-ontologies.com/bot#Zone
<http://www.owl-ontologies.com/bot#Zone> rdf:type owl:Class .


###  http://www.owl-ontologies.com/geo#Feature
<http://www.owl-ontologies.com/geo#Feature> rdf:type owl:Class ;
                                            rdfs:label "Feature" .


###  http://www.owl-ontologies.com/quantityKind#AmountOfSubstanceConcentration
<http://www.owl-ontologies.com/quantityKind#AmountOfSubstanceConcentration> rdf:type owl:Class ;
                                                                            rdfs:label "Amount Of Substance Concentration" .


###  http://www.owl-ontologies.com/quantityKind#Density
<http://www.owl-ontologies.com/quantityKind#Density> rdf:type owl:Class ;
                                                     rdfs:label "Density" .


###  http://www.owl-ontologies.com/quantityKind#PersonCount
<http://www.owl-ontologies.com/quantityKind#PersonCount> rdf:type owl:Class ;
                                                         rdfs:label "Person Count" .


###  http://www.owl-ontologies.com/quantityKind#VolumetricFlowRate
<http://www.owl-ontologies.com/quantityKind#VolumetricFlowRate> rdf:type owl:Class ;
                                                                rdfs:label "Volumetric Flow Rate" .


###  http://www.owl-ontologies.com/sosa#Actuation
<http://www.owl-ontologies.com/sosa#Actuation> rdf:type owl:Class ;
                                               rdfs:label "Actuation" .


###  http://www.owl-ontologies.com/sosa#FeatureOfInterest
<http://www.owl-ontologies.com/sosa#FeatureOfInterest> rdf:type owl:Class ;
                                                       rdfs:label "Feature Of Interest" .


###  http://www.owl-ontologies.com/sosa#Observation
<http://www.owl-ontologies.com/sosa#Observation> rdf:type owl:Class .


###  http://www.owl-ontologies.com/sosa#Procedure
<http://www.owl-ontologies.com/sosa#Procedure> rdf:type owl:Class ;
                                               rdfs:label "Procedure" .


###  http://www.owl-ontologies.com/time#Instant
<http://www.owl-ontologies.com/time#Instant> rdf:type owl:Class .


###  http://www.owl-ontologies.com/time#Interval
<http://www.owl-ontologies.com/time#Interval> rdf:type owl:Class .


#################################################################
#    Individuals
#################################################################

###  http://www.owl-ontologies.com/BIMxel#AnonymizePeople
<http://www.owl-ontologies.com/BIMxel#AnonymizePeople> rdf:type owl:NamedIndividual ;
                                                       rdfs:comment "Ensures that individuals’ identities cannot be recognized, even using image sensors, to comply with privacy regulations."@en ;
                                                       rdfs:label "Evitar en origen la identidad de las personas"@es ,
                                                                  "Prevent identification of people at source"@en .


###  http://www.owl-ontologies.com/BIMxel#AverageCO2Levels
<http://www.owl-ontologies.com/BIMxel#AverageCO2Levels> rdf:type owl:NamedIndividual ;
                                                        rdfs:comment "Measures the average carbon dioxide (CO2) levels in ppm. An indicator of air quality and ventilation."@en ;
                                                        rdfs:label "Average carbon dioxide levels in ppm"@en ,
                                                                   "Niveles de dióxido de carbono medios en ppm"@es .


###  http://www.owl-ontologies.com/BIMxel#CO2EvolutionPatterns
<http://www.owl-ontologies.com/BIMxel#CO2EvolutionPatterns> rdf:type owl:NamedIndividual ;
                                                            rdfs:comment "Analyzes how CO2 levels vary throughout the day. Helps optimize ventilation and detect occupancy peaks."@en ;
                                                            rdfs:label "CO2 level evolution patterns throughout the day"@en ,
                                                                       "Patrones de evolución de los niveles de CO2 a lo largo del día"@es .


###  http://www.owl-ontologies.com/BIMxel#CondensationDetectionCritical
<http://www.owl-ontologies.com/BIMxel#CondensationDetectionCritical> rdf:type owl:NamedIndividual ;
                                                                     rdfs:comment "Detects condensation in critical areas (walls, ceilings, sensitive equipment). Helps prevent structural damage or equipment failure."@en ;
                                                                     rdfs:label "Detección de condensación en áreas críticas"@es ,
                                                                                "Detection of condensation in critical areas"@en .


###  http://www.owl-ontologies.com/BIMxel#ConsumptionPeaks
<http://www.owl-ontologies.com/BIMxel#ConsumptionPeaks> rdf:type owl:NamedIndividual ;
                                                        rdfs:comment "Identifies moments of maximum energy consumption, useful for demand management and peak reduction."@en ;
                                                        rdfs:label "Consumption peaks"@en ,
                                                                   "Picos de consumo"@es .


###  http://www.owl-ontologies.com/BIMxel#EnergyConsumptionByEquipment
<http://www.owl-ontologies.com/BIMxel#EnergyConsumptionByEquipment> rdf:type owl:NamedIndividual ;
                                                                    rdfs:comment "Measures energy consumption per specific equipment, helping detect inefficient or faulty devices."@en ;
                                                                    rdfs:label "Consumo por equipos"@es ,
                                                                               "Energy consumption by equipment"@en .


###  http://www.owl-ontologies.com/BIMxel#EnergyConsumptionBySpace
<http://www.owl-ontologies.com/BIMxel#EnergyConsumptionBySpace> rdf:type owl:NamedIndividual ;
                                                                rdfs:comment "Measures energy consumption by zone or space, allowing identification of high-consumption areas and improving efficiency."@en ;
                                                                rdfs:label "Consumo por espacios"@es ,
                                                                           "Energy consumption by spaces"@en .


###  http://www.owl-ontologies.com/BIMxel#EquipmentTemperatures
<http://www.owl-ontologies.com/BIMxel#EquipmentTemperatures> rdf:type owl:NamedIndividual ;
                                                             rdfs:comment "Records the temperature of specific equipment, such as servers, machinery, or HVAC systems, to prevent overheating and maintain efficiency."@en ;
                                                             rdfs:label "Temperaturas de equipos específicos"@es ,
                                                                        "Temperatures of specific equipment"@en .


###  http://www.owl-ontologies.com/BIMxel#IndoorAmbientTemperature
<http://www.owl-ontologies.com/BIMxel#IndoorAmbientTemperature> rdf:type owl:NamedIndividual ;
                                                                rdfs:comment "Measures the air temperature inside a building or space. Useful for controlling thermal comfort and HVAC efficiency."@en ;
                                                                rdfs:label "Indoor ambient temperature"@en ,
                                                                           "Temperatura ambiental interior"@es .


###  http://www.owl-ontologies.com/BIMxel#IndoorRelativeHumidity
<http://www.owl-ontologies.com/BIMxel#IndoorRelativeHumidity> rdf:type owl:NamedIndividual ;
                                                              rdfs:comment "Indicates the relative humidity indoors. Important for human comfort, material preservation, and mold prevention."@en ;
                                                              rdfs:label "Humedad relativa del aire interior"@es ,
                                                                         "Indoor air relative humidity"@en .


###  http://www.owl-ontologies.com/BIMxel#OccupancyLevel
<http://www.owl-ontologies.com/BIMxel#OccupancyLevel> rdf:type owl:NamedIndividual ;
                                                      rdfs:comment "Indicates the number or percentage of occupants in a space at a given time, useful for resource management and safety."@en ;
                                                      rdfs:label "Nivel de ocupación"@es ,
                                                                 "Occupancy level"@en .


###  http://www.owl-ontologies.com/BIMxel#OccupancyPatterns
<http://www.owl-ontologies.com/BIMxel#OccupancyPatterns> rdf:type owl:NamedIndividual ;
                                                         rdfs:comment "Identifies occupancy patterns over time, useful for scheduling, energy management, and cleaning planning."@en ;
                                                         rdfs:label "Identificar patrones de ocupación"@es ,
                                                                    "Identify occupancy patterns"@en .


###  http://www.owl-ontologies.com/BIMxel#OutdoorAmbientTemperature
<http://www.owl-ontologies.com/BIMxel#OutdoorAmbientTemperature> rdf:type owl:NamedIndividual ;
                                                                 rdfs:comment "Measures the air temperature inside a building or space. Useful for controlling thermal comfort and HVAC efficiency."@en ;
                                                                 rdfs:label "Outdoor ambient temperature"@en ,
                                                                            "Temperatura ambiental exterior"@es .


###  http://www.owl-ontologies.com/BIMxel#OutdoorRelativeHumidity
<http://www.owl-ontologies.com/BIMxel#OutdoorRelativeHumidity> rdf:type owl:NamedIndividual ;
                                                               rdfs:comment "Indicates the relative humidity of outdoor air, useful for planning ventilation and adjusting HVAC systems according to external conditions."@en ;
                                                               rdfs:label "Humedad relativa del aire exterior"@es ,
                                                                          "Outdoor air relative humidity"@en .


###  http://www.owl-ontologies.com/BIMxel#PeopleCountImageDetection
<http://www.owl-ontologies.com/BIMxel#PeopleCountImageDetection> rdf:type owl:NamedIndividual ;
                                                                 rdfs:comment "Detects the number of people present using images, while preserving privacy. Facilitates occupancy management and flow analysis."@en ;
                                                                 rdfs:label "Detección por imagen del número de personas presentes"@es ,
                                                                            "Image-based detection of number of people present"@en .


###  http://www.owl-ontologies.com/BIMxel#PresenceDetection
<http://www.owl-ontologies.com/BIMxel#PresenceDetection> rdf:type owl:NamedIndividual ;
                                                         rdfs:comment "Detects whether people are present in an area without counting each individual. Useful for lighting, HVAC, or security control."@en ;
                                                         rdfs:label "Detección de presencia"@es ,
                                                                    "Presence detection"@en .


###  http://www.owl-ontologies.com/BIMxel#RealTimeLeakDetection
<http://www.owl-ontologies.com/BIMxel#RealTimeLeakDetection> rdf:type owl:NamedIndividual ;
                                                             rdfs:comment "Detects water leaks in real time, helping prevent waste and damage."@en ;
                                                             rdfs:label "Detección de fugas en tiempo real"@es ,
                                                                        "Real-time leak detection"@en .


###  http://www.owl-ontologies.com/BIMxel#StandbyOrPhantomPowerDevices
<http://www.owl-ontologies.com/BIMxel#StandbyOrPhantomPowerDevices> rdf:type owl:NamedIndividual ;
                                                                    rdfs:comment "Detects devices in standby mode or consuming “phantom” power, to reduce energy waste."@en ;
                                                                    rdfs:label "Identificación de dispositivos en modo de espera o con consumo fantasma"@es ,
                                                                               "Identification of devices in standby or phantom power"@en .


###  http://www.owl-ontologies.com/BIMxel#TemperatureGradientLevels
<http://www.owl-ontologies.com/BIMxel#TemperatureGradientLevels> rdf:type owl:NamedIndividual ;
                                                                 rdfs:comment "Measures how temperature changes at different heights or levels within a space (e.g., floor to ceiling). Helps identify air stratification."@en ;
                                                                 rdfs:label "Gradiente de temperatura en diferentes niveles"@es ,
                                                                            "Temperature gradient at different levels"@en .


###  http://www.owl-ontologies.com/BIMxel#ThermalVariationsByZone
<http://www.owl-ontologies.com/BIMxel#ThermalVariationsByZone> rdf:type owl:NamedIndividual ;
                                                               rdfs:comment "Records temperature differences between different zones or rooms in a building. Helps detect thermal imbalances or heating/cooling issues."@en ;
                                                               rdfs:label "Thermal variations by zones or rooms"@en ,
                                                                          "Variaciones térmicas por zonas o habitaciones"@es .


###  http://www.owl-ontologies.com/BIMxel#TotalEnergyConsumption
<http://www.owl-ontologies.com/BIMxel#TotalEnergyConsumption> rdf:type owl:NamedIndividual ;
                                                              rdfs:comment "Measures the total energy consumption of the building over a period, for monitoring and cost reduction."@en ;
                                                              rdfs:label "Consumo energético total del edificio"@es ,
                                                                         "PTotal energy consumption of the building"@en .


###  http://www.owl-ontologies.com/BIMxel#TotalWaterUsage
<http://www.owl-ontologies.com/BIMxel#TotalWaterUsage> rdf:type owl:NamedIndividual ;
                                                       rdfs:comment "Measures the total volume of water used over a period, useful for consumption control and sustainability."@en ;
                                                       rdfs:label "Total water usage"@en ,
                                                                  "Volumen total de agua utilizada"@es .


###  http://www.owl-ontologies.com/BIMxel#VentilationDeficiencies
<http://www.owl-ontologies.com/BIMxel#VentilationDeficiencies> rdf:type owl:NamedIndividual ;
                                                               rdfs:comment "Identifies areas or situations with insufficient ventilation, which may affect air quality and occupant health."@en ;
                                                               rdfs:label "Identificar deficiencias en la ventilación"@es ,
                                                                          "Identify ventilation deficiencies"@en .


###  http://www.owl-ontologies.com/BIMxel#WaterConsumptionByZone
<http://www.owl-ontologies.com/BIMxel#WaterConsumptionByZone> rdf:type owl:NamedIndividual ;
                                                              rdfs:comment "Measures water usage by zone or type of use (bathrooms, kitchens, irrigation), to optimize resources and detect anomalies."@en ;
                                                              rdfs:label "Consumo por zonas o tipos de uso"@es ,
                                                                         "Water consumption by zones or type of use"@en .


###  http://www.owl-ontologies.com/BIMxel#WaterFlowAnalysisByTime
<http://www.owl-ontologies.com/BIMxel#WaterFlowAnalysisByTime> rdf:type owl:NamedIndividual ;
                                                               rdfs:comment "Analyzes water flow at different times, allowing identification of consumption peaks or unusual patterns."@en ;
                                                               rdfs:label "Analysis of water flow at different times"@en ,
                                                                          "Análisis del flujo de agua en diferentes horarios"@es .


###  http://www.owl-ontologies.com/BIMxel#WaterLevelsTanks
<http://www.owl-ontologies.com/BIMxel#WaterLevelsTanks> rdf:type owl:NamedIndividual ;
                                                        rdfs:comment "Measures water levels in tanks or reservoirs, useful for supply management and refill planning."@en ;
                                                        rdfs:label "Niveles de agua en tanques o depósitos"@es ,
                                                                   "Water levels in tanks or reservoirs"@en .


###  http://www.owl-ontologies.com/bimxel#BIMxel_IndoorAmbientTemperature
:BIMxel_IndoorAmbientTemperature rdf:type owl:NamedIndividual .


#################################################################
#    Annotations
#################################################################

<http://www.owl-ontologies.com/bot#Element> rdfs:label "Element" ,
                                                       "element" .


<http://www.owl-ontologies.com/bot#Space> rdfs:label "Space" ,
                                                     "space" .


<http://www.owl-ontologies.com/bot#Zone> rdfs:label "Zone" ,
                                                    "zone" .


<http://www.owl-ontologies.com/sosa#Observation> rdfs:label "Observation" ,
                                                            "observation" .


<http://www.owl-ontologies.com/time#Instant> rdfs:label "Instant" ,
                                                        "instant" .


<http://www.owl-ontologies.com/time#Interval> rdfs:label "Interval" ,
                                                         "interval" .


###  Generated by the OWL API (version 5.1.18) https://github.com/owlcs/owlapi/
